1) proved the reachablity algorithm is complete w.r.t the declarative version, and also moved its definition to Vellvm.
For mem2reg, we do not need its soundness (which GVN needs).
Completeness is by induction of graphs. Soundness should be by induction
of Kildall algorithm, which we will show in the later proofs.

2) split dtree.v into dtree.v (definitions) and dtree_props.v
(properties). mem2reg only needs dtree.v, GVN needs both of them.
dtree_props.v includes two admitted lemmas: one is the soundness of
reachablity, the other is a trivial infrastructure lemma. Removed all
the dependence to dtree_props.v from mem2reg proofs. So mem2reg does not
reply on the two unproved lemmas.



git-svn-id: https://webdav.seas.upenn.edu/svn/sol/vol@3903 eef5ea85-cc2e-0410-bd84-0fae1f012da8

src3.0/Vellvm/analysis.v
@@ -135,6 +135,26 @@ Definition areachable (f: fdef) : AMap.t bool :=
   | Some rs => rs
   end.
 
+Fixpoint get_reachable_labels (bd:list l) (rd:AMap.t bool) (acc:list l)
+  : list l :=
+match bd with
+| nil => acc
+| l0::bd' => if (AMap.get l0 rd)
+             then get_reachable_labels bd' rd (l0::acc)
+             else get_reachable_labels bd' rd acc
+end.
+
+Definition reachablity_analysis (f: fdef) : option (list l) :=
+match getEntryBlock f with
+| Some (block_intro root _ _ _) =>
+    let 'bd := bound_fdef f in
+    match areachable_aux f with
+    | None => None
+    | Some rd => Some (get_reachable_labels bd rd nil)
+    end
+| None => None
+end.
+
 Require Import Dipaths.
 
 Definition vertexes_fdef (f:fdef) : V_set :=
@@ -749,6 +769,59 @@ Proof.
       eapply successors__blockInFdefB; eauto.
     destruct J as [ps0 [cs0 [tmn0 [HBinF' Hinsucc]]]].
     eapply areachable_successors; eauto.
+Qed.
+
+Lemma reachable__in_bound: forall f a (Hrd: reachable f a),
+  In a (bound_fdef f).
+Proof.
+  intros.
+  unfold reachable in Hrd.
+  match goal with
+  | H: match ?e with
+       | Some _ => _
+       | None => is_true false
+       end |- _ => remember e as R; destruct R; tinv H
+  end.
+  destruct b.
+  destruct Hrd as [vl [al Hrd]].
+  apply Dipaths.DW_endx_inv in Hrd. auto.
+Qed.
+
+Lemma get_reachable_labels__spec_aux: forall a (t:AMap.t bool)
+  (Hin : t !! a) bnd acc (Hinbnd : In a bnd \/ In a acc),
+  In a (get_reachable_labels bnd t acc).
+Proof.
+  induction bnd; simpl; intros; try tauto.
+    destruct Hinbnd as [[EQ | Hinbnd] | Hinbnd]; subst.
+      rewrite Hin.
+      apply IHbnd; simpl; auto.
+
+      destruct_if; auto.
+      destruct_if; auto.
+        apply IHbnd; simpl; auto.
+Qed.
+
+Lemma get_reachable_labels__spec: forall a (t:AMap.t bool) bnd
+  (Hin : t !! a) (Hinbnd : In a bnd),
+  In a (get_reachable_labels bnd t nil).
+Proof.
+  intros.
+  apply get_reachable_labels__spec_aux; simpl; auto.
+Qed.
+
+Lemma reachable__reachablity_analysis: forall f rd a
+  (Huniq: uniqFdef f) (Hdec: reachable f a)
+  (Halg: reachablity_analysis f = Some rd),
+  In a rd.
+Proof.
+  intros.
+  assert (Hinbnd:=Hdec).
+  apply reachable__in_bound in Hinbnd.
+  apply areachable_is_correct in Hdec; auto.
+  unfold reachablity_analysis in Halg.
+  inv_mbind. destruct b as [l0 ps0 cs0 tmn0]. inv_mbind.
+  unfold areachable in Hdec. rewrite <- HeqR0 in Hdec.
+  apply get_reachable_labels__spec; auto.
 Qed.
 
 Lemma arcs_fdef_inv : forall f a1 a2,
