src3.0/Transforms/mem2reg.v
@@ -4,9 +4,8 @@ Require Import ListSet.
 Require Import Maps.
 Require Import Lattice.
 Require Import Iteration.
-Require Import dtree.
 Require Import primitives.
-Require Import Maps.
+Require Import dtree.
 
 Record vmap := mkVMap {
   alloca: value;
